theories/binders/DeBruijn_CPS.v
@@ -1,0 +1,459 @@
+From Stdlib Require Import Bool Nat List Lia.
+From Stdlib.Classes Require Import Morphisms.
+Import ListNotations.
+
+(** If [H] is a hypothesis [H : P -> Q], [feed H] first asks to prove [P],
+    and then the original goal with [H : Q]. *)
+
+Ltac feed_aux H :=
+  match type of H with
+  | ?P -> ?Q =>
+    let HP := fresh "H" in
+    assert P as HP ; [| specialize (H HP) ; clear HP ]
+  end.
+
+Tactic Notation "feed" ident(H) "by" tactic3(t) :=
+  feed_aux H ; [now t|].
+
+Tactic Notation "feed" ident(H) :=
+  feed_aux H.
+
+(**************************************************************************)
+(** *** lambda terms. *)
+(**************************************************************************)
+
+(** Untyped lambda terms, using de Bruijn indices. *)
+Inductive term :=
+| var : nat -> term
+| app : term -> term -> term
+| lam : term -> term
+| letin : term -> term -> term.
+
+(** [apps f xs] forms the n-ary application of [f] to arguments [xs]. *)
+Fixpoint apps (f : term) (xs : list term) : term :=
+  match xs with
+  | [] => f
+  | x :: xs => apps (app f x) xs
+  end.
+
+(**************************************************************************)
+(** *** Renamings. *)
+(**************************************************************************)
+
+(** A renaming is a map from de Bruijn indices to de Bruijn indices. *)
+Definition ren := nat -> nat.
+
+Definition rid : ren :=
+  fun i => i.
+
+Definition rshift : ren :=
+  fun i => S i.
+
+Definition rcons (i : nat) (r : ren) : ren :=
+  fun i' =>
+    match i' with
+    | 0 => i
+    | S i' => r i'
+    end.
+
+Definition rcomp (r1 r2 : ren) : ren :=
+  fun i => r2 (r1 i).
+
+Definition rup (r : ren) : ren :=
+  rcons 0 (rcomp r rshift).
+
+(** [lift0 ofs] is a renaming which adds [ofs] to every index. *)
+Fixpoint lift0 (ofs : nat) : ren :=
+  match ofs with
+  | 0 => rid
+  | S ofs => rcomp rshift (lift0 ofs)
+  end.
+
+(** [lift base ofs] is a renaming which adds [ofs] to every index
+    greater or equal to [base]. *)
+Fixpoint lift (base ofs : nat) : ren :=
+  match base with
+  | 0 => lift0 ofs
+  | S base => rup (lift base ofs)
+  end.
+
+(** [rename r t] applies renaming [r] to term [t]. *)
+Fixpoint rename (r : ren) (t : term) : term :=
+  match t with
+  | var i => var (r i)
+  | app t1 t2 => app (rename r t1) (rename r t2)
+  | lam t => lam (rename (rup r) t)
+  | letin t u => letin (rename r t) (rename (rup r) u)
+  end.
+
+(**************************************************************************)
+(** *** Contexts and well-scoped terms. *)
+(**************************************************************************)
+
+Inductive ldecl :=
+| LAssum : ldecl
+| LDef : term -> ldecl.
+
+Definition context := list ldecl.
+
+(** [scoping n t] states that [t] every de Bruijn index in [t]
+    is smaller than [n]. *)
+Inductive scoping : nat -> term -> Prop :=
+| scoping_var n i :
+    i < n -> scoping n (var i)
+| scoping_app n t1 t2 :
+    scoping n t1 ->
+    scoping n t2 ->
+    scoping n (app t1 t2)
+| scoping_lam n t :
+    scoping (S n) t ->
+    scoping n (lam t)
+| scoping_letin n t u :
+    scoping n t ->
+    scoping (S n) u ->
+    scoping n (letin t u).
+
+#[export] Hint Resolve scoping_var scoping_app scoping_lam scoping_letin : scoping.
+#[export] Hint Extern 10 (_ < _) => lia : scoping.
+
+Lemma scoping_var_zero n :
+  scoping (S n) (var 0).
+Proof. constructor. lia. Qed.
+
+Lemma scoping_var_succ n i :
+  scoping n (var i) -> scoping (S n) (var (S i)).
+Proof. constructor. inversion H ; subst. lia. Qed.
+
+#[export] Hint Resolve scoping_var_zero scoping_var_succ : scoping.
+
+Lemma scoping_weaken n n' t :
+  n <= n' -> scoping n t -> scoping n' t.
+Proof.
+intros Hn H. induction H in n', Hn |- *.
+- constructor. lia.
+- constructor ; auto.
+- constructor. apply IHscoping. lia.
+- constructor.
+  + apply IHscoping1. assumption.
+  + apply IHscoping2. lia.
+Qed.
+
+Lemma scoping_weaken_one n t :
+  scoping n t -> scoping (S n) t.
+Proof. apply scoping_weaken ; lia. Qed.
+#[export] Hint Resolve scoping_weaken_one : scoping.
+
+(** [rscoping n1 n2 r] states that [r] maps a context of size [n1]
+    into a context of size [n2]. *)
+Definition rscoping (n1 n2 : nat) (r : ren) : Prop :=
+  forall i, i < n1 -> r i < n2.
+
+Lemma rscoping_rid n :
+  rscoping n n rid.
+Proof. intros i Hi. unfold rid. lia. Qed.
+
+Lemma rscoping_rshift n :
+  rscoping n (S n) rshift.
+Proof. intros i Hi. unfold rshift. lia. Qed.
+
+Lemma rscoping_rcomp n1 n2 n3 r r' :
+  rscoping n1 n2 r ->
+  rscoping n2 n3 r' ->
+  rscoping n1 n3 (rcomp r r').
+Proof. intros H1 H2 i Hi. unfold rcomp. apply H2, H1. assumption. Qed.
+
+Lemma rscoping_rcons n1 n2 i r :
+  i < n2 ->
+  rscoping n1 n2 r ->
+  rscoping (S n1) n2 (rcons i r).
+Proof. *
+intros H1 H2 [|j] Hj ; cbn.
+- assumption.
+- apply H2. lia.
+Qed.
+
+#[export] Hint Resolve rscoping_rid rscoping_rshift rscoping_rcomp rscoping_rcons : scoping.
+#[export] Hint Unfold rup : scoping.
+
+(** Scoping is preserved by renaming. *)
+Lemma scoping_rename r t n1 n2 :
+  scoping n1 t ->
+  rscoping n1 n2 r ->
+  scoping n2 (rename r t).
+Proof.
+intros Ht Hr. induction Ht in r, Hr, n2 |- * ; cbn.
+- constructor. now apply Hr.
+- constructor.
+  + now apply IHHt1.
+  + now apply IHHt2.
+- constructor. apply IHHt. intros i Hi. destruct i as [|i] ; cbn in *.
+  + lia.
+  + unfold rcomp, rshift. rewrite <-PeanoNat.Nat.succ_lt_mono. apply Hr. lia.
+- constructor.
+  + now apply IHHt1.
+  + apply IHHt2. intros i Hi. destruct i as [|i] ; cbn in *.
+    * lia.
+    * unfold rcomp, rshift. rewrite <-PeanoNat.Nat.succ_lt_mono. apply Hr. lia.
+Qed.
+
+#[export] Hint Resolve scoping_rename : scoping.
+
+(**************************************************************************)
+(** *** Monadic programs. *)
+(**************************************************************************)
+
+(** Our monad [M] allows several effects:
+    - read/write access to a local context.
+    - critical failure.
+    - out of fuel, which is not considered a failure. *)
+
+Inductive result (A : Type) : Type :=
+| Success (x : A) : result A
+| Error : result A
+| OutOfFuel : result A.
+Arguments Success {A} x.
+Arguments Error {A}.
+Arguments OutOfFuel {A}.
+
+Definition M (A : Type) : Type :=
+  context -> result (context * A).
+
+Definition ret {A} (x : A) : M A :=
+  fun ctx => Success (ctx, x).
+
+Definition bind {A B} (mx : M A) (f : A -> M B) : M B :=
+  fun ctx =>
+    match mx ctx with
+    | Success (ctx, x) => f x ctx
+    | OutOfFuel => OutOfFuel
+    | Error => Error
+    end.
+
+Notation "x >>= f" := (bind x f) (at level 50, no associativity).
+Notation "f =<< x" := (bind x f) (at level 50, no associativity).
+
+(** [let*] monadic notation. *)
+Notation "'let*' x ':=' t 'in' u" := (bind t (fun x => u))
+  (at level 100, right associativity, t at next level, x pattern).
+
+Definition fmap {A B} (f : A -> B) (mx : M A) : M B :=
+  let* x := mx in
+  ret (f x).
+
+Notation "f <$> x" := (fmap f x) (at level 30, right associativity).
+
+(** Signal fuel is out. *)
+Definition out_of_fuel {A} : M A := fun ctx => OutOfFuel.
+
+(** Fail. *)
+Definition error {A} : M A := fun ctx => Error.
+
+(** Read the local context. *)
+Definition get_ctx : M context :=
+  fun ctx => Success (ctx, ctx).
+
+(** Replace the local context. *)
+Definition put_ctx (ctx : context) : M unit :=
+  fun _ => Success (ctx, tt).
+
+(** Extend the local context with a new local declaration,
+    run a computation, and restore the local context. *)
+Definition with_decl {A} (d : ldecl) (m : M A) : M A :=
+  let* ctx := get_ctx in
+  let* _ := put_ctx (d :: ctx) in
+  let* a := m in
+  let* _ := put_ctx ctx in
+  ret a.
+
+(** Convenience function to build a lambda abstraction. *)
+Definition mk_lambda (f : M term) : M term :=
+  with_decl LAssum
+    (let* body := f in
+     ret (lam body)).
+
+(** Convenience function to build a let-expression. *)
+Definition mk_letin (def : term) (f : M term) : M term :=
+  with_decl (LDef def)
+    (let* body := f in
+     ret (letin def body)).
+
+(**************************************************************************)
+(** *** Program logic. *)
+(**************************************************************************)
+
+(** Weakest-precondition: [wp ctx m Q] means that running [m] in initial
+    context [ctx] will not raise an error (out of fuel is fine), and the
+    return value and final context satisfy [Q]. *)
+Definition wp {A} (ctx1 : context) (m : M A) (Q : context -> A -> Prop) : Prop :=
+  match m ctx1 with
+  | OutOfFuel => True
+  | Error => False
+  | Success (ctx2, a) => Q ctx2 a
+  end.
+
+Lemma wp_ret {A} ctx (a : A) Q :
+  Q ctx a -> wp ctx (ret a) Q.
+Proof. intros H. cbn. assumption. Qed.
+
+Lemma wp_bind {A B} ctx (m : M A) (f : A -> M B) Q :
+  wp ctx m (fun ctx' a => wp ctx' (f a) Q) -> wp ctx (let* x := m in f x) Q.
+Proof.
+cbv. destruct (m ctx) as [[ctx' a] | |] ; cbn ; intros H ; [| auto..].
+destruct (f a ctx') as [[ctx'' b] | |] ; auto.
+Qed.
+
+Lemma wp_fmap {A B} ctx (f : A -> B) (mx : M A) Φ :
+  wp ctx mx (fun ctx x => Φ ctx (f x)) -> wp ctx (fmap f mx) Φ.
+Proof. intros H. unfold fmap. apply wp_bind. apply H. Qed.
+
+Lemma wp_consequence {A} ctx (m : M A) Q Q' :
+  (forall a ctx', Q a ctx' -> Q' a ctx') -> wp ctx m Q -> wp ctx m Q'.
+Proof.
+intros H1. cbv. destruct (m ctx) as [[ctx' a] | |] ; cbn ; intros H ; [| auto..].
+apply H1. assumption.
+Qed.
+
+Lemma wp_out_of_fuel {A} ctx Φ : wp ctx (@out_of_fuel A) Φ.
+Proof. cbn. constructor. Qed.
+
+Lemma wp_put ctx ctx' Φ :
+  Φ ctx' tt -> wp ctx (put_ctx ctx') Φ.
+Proof. cbn. auto. Qed.
+
+Lemma wp_get ctx Φ :
+  Φ ctx ctx -> wp ctx get_ctx Φ.
+Proof. cbn. auto. Qed.
+
+Lemma wp_with_decl {A} ctx Φ d (m : M A) :
+  wp (d :: ctx) m (fun _ a => Φ ctx a) -> wp ctx (with_decl d m) Φ.
+Proof. cbv. destruct (m (d :: ctx)) as [[a ctx'] | |] ; auto. Qed.
+
+Lemma wp_mk_lambda f ctx Φ :
+  (wp (LAssum :: ctx) f (fun _ body => Φ ctx (lam body))) ->
+  wp ctx (mk_lambda f) Φ.
+Proof.
+intros H. unfold mk_lambda. apply wp_with_decl, wp_bind. apply H.
+Qed.
+
+Lemma wp_mk_letin def f ctx Φ :
+  (wp (LDef def :: ctx) f (fun _ body => Φ ctx (letin def body))) ->
+  wp ctx (mk_letin def f) Φ.
+Proof.
+intros H. unfold mk_letin. apply wp_with_decl, wp_bind. apply H.
+Qed.
+
+Ltac wp_step :=
+  match goal with
+  | [ |- wp _ (ret _) _ ] => apply wp_ret
+  | [ |- wp _ (bind _ _) _ ] => apply wp_bind
+  | [ |- wp _ (fmap _ _) _ ] => apply wp_fmap
+  | [ |- wp _ out_of_fuel _ ] => apply wp_out_of_fuel
+  | [ |- wp _ get_ctx _ ] => apply wp_get
+  | [ |- wp _ (put_ctx _) _ ] => apply wp_put
+  | [ |- wp _ (with_decl _ _) _ ] => apply wp_with_decl
+  | [ |- wp _ (mk_lambda _) _ ] => apply wp_mk_lambda
+  | [ |- wp _ (mk_letin _ _) _ ] => apply wp_mk_letin
+  end.
+
+Ltac wp_steps := repeat wp_step.
+
+(** Hoare triples. *)
+Definition hoare_triple {A} (P : context -> Prop) (m : M A) (Q : context -> A -> Prop) : Prop :=
+  forall ctx, forall Φ, P ctx -> (forall a, Q ctx a -> Φ ctx a) -> wp ctx m Φ.
+
+(** Hoare triple. *)
+Notation "'{{' c1 '.' P '}}' m '{{' c2 v '.' Q '}}'" :=
+  (hoare_triple (fun c1 => P) m (fun c2 v => Q))
+  (at level 100, c1 binder, v binder, c2 binder).
+
+(** Prove a goal of the form [scoping _ _].
+    Succeeds or does nothing. *)
+Ltac prove_scoping :=
+  match goal with
+  | [ |- scoping _ _ ] =>
+    solve [ cbn in * ; autounfold with scoping ; eauto 10 with scoping ]
+  end.
+
+(**************************************************************************)
+(** *** CPS transformation meta-program. *)
+(**************************************************************************)
+
+Fixpoint cps (n : nat) (t : term) (k : term) : M term :=
+  match n with 0 => out_of_fuel | S n =>
+  match t with
+  | var i => ret (app k (var i))
+  | app t1 t2 =>
+    cps n t1 =<< mk_lambda ( (* x1 *)
+    cps n (rename (lift0 1) t2) =<< mk_lambda ( (* x2 *)
+    ret (apps (var 1 (* x1 *)) [ var 0 (* x2 *) ; rename (lift0 2) k ])))
+  | lam t' =>
+    app k <$>
+      mk_lambda ( (* x *)
+      mk_lambda ( (* k' *)
+      cps n (rename (lift0 1) t') (var 0 (* k' *))))
+  | letin t u =>
+    cps n t =<< mk_lambda ( (* v *)
+    mk_letin (var 0 (* v *)) ( (* x *)
+    cps n (rename (lift 1 1) u) (rename (lift0 2) k)))
+  end
+  end.
+
+Lemma cps_safe n t k :
+  {{ ctx. scoping (length ctx) t /\ scoping (length ctx) k }}
+    cps n t k
+  {{ ctx t'. scoping (length ctx) t' }}.
+Proof.
+induction n in k, t |- * ; intros ctx Φ [Ht Hk] HΦ ; cbn ; [constructor|].
+destruct t ; cbn.
+- apply HΦ. prove_scoping.
+- inversion Ht ; subst. wp_steps.
+  apply IHn. { split ; prove_scoping. }
+  intros t' Ht'. apply IHn. { split ; prove_scoping. }
+  intros t'' Ht''. apply HΦ. assumption.
+- wp_steps. apply IHn. { inversion Ht ; subst. split ; prove_scoping. }
+  intros t' Ht'. wp_steps. apply HΦ. prove_scoping.
+- inversion Ht ; subst. wp_steps.
+  apply IHn. { split ; prove_scoping. }
+  intros t' Ht'. apply IHn. { split ; prove_scoping. }
+  intros t'' Ht''. apply HΦ. assumption.
+Qed.
+
+
+(**************************************************************************)
+(** *** CPS transformation, second version. *)
+(**************************************************************************)
+
+Inductive red : term -> term -> Prop :=
+| red_beta :
+
+
+(**
+Γ |- t
+r : Γ -> Δ
+k : Δ
+
+Γ, x |- t
+------------
+Γ |- mk_lambda t
+
+*)
+
+Fixpoint cps2 (n : nat) (r : ren) (t : term) (k : term) : M term :=
+  match n with 0 => out_of_fuel | S n =>
+  match t with
+  | var i => ret (app k (var (r i)))
+  | app t1 t2 =>
+    cps n r t1 =<< mk_lambda ( (* x1 *)
+    cps n (rcomp r (lift0 1)) t2 =<< mk_lambda ( (* x2 *)
+    ret (apps (var 1 (* x1 *)) [ var 0 (* x2 *) ; rename (lift0 2) k ])))
+  | lam t' =>
+    app k <$>
+      mk_lambda ( (* x *)
+      mk_lambda ( (* k' *)
+      cps n (rename (lift0 1) t') (var 0 (* k' *))))
+  | letin t u =>
+    cps n t =<< mk_lambda ( (* v *)
+    mk_letin (var 0 (* v *)) ( (* x *)
+    cps n (rename (lift 1 1) u) (rename (lift0 2) k)))
+  end
+  end.
