theories/binders/Weituo_CPS.v
@@ -1,0 +1,252 @@
+From Stdlib Require Import Bool Nat List String Lia.
+From Stdlib.Classes Require Import Morphisms.
+From stdpp Require Import gmap.
+Import ListNotations.
+
+(** If [H] is a hypothesis [H : P -> Q], [feed H] first asks to prove [P],
+    and then the original goal with [H : Q]. *)
+
+Ltac feed_aux H :=
+  match type of H with
+  | ?P -> ?Q =>
+    let HP := fresh "H" in
+    assert P as HP ; [| specialize (H HP) ; clear HP ]
+  end.
+
+Tactic Notation "feed" ident(H) "by" tactic3(t) :=
+  feed_aux H ; [now t|].
+
+Tactic Notation "feed" ident(H) :=
+  feed_aux H.
+
+(**************************************************************************)
+(** *** lambda terms. *)
+(**************************************************************************)
+
+(** Untyped lambda terms, using de Bruijn indices. *)
+Inductive term :=
+| var : nat -> term
+| app : term -> term -> term
+| lam : term -> term
+| letin : term -> term -> term.
+
+(** [apps f xs] forms the n-ary application of [f] to arguments [xs]. *)
+Fixpoint apps (f : term) (xs : list term) : term :=
+  match xs with
+  | [] => f
+  | x :: xs => apps (app f x) xs
+  end.
+
+(**************************************************************************)
+(** *** Renamings. *)
+(**************************************************************************)
+
+(** A renaming is a map from de Bruijn indices to de Bruijn indices. *)
+Definition ren := nat -> nat.
+
+Definition rid : ren :=
+  fun i => i.
+
+Definition rshift : ren :=
+  fun i => S i.
+
+Definition rcons (i : nat) (r : ren) : ren :=
+  fun i' =>
+    match i' with
+    | 0 => i
+    | S i' => r i'
+    end.
+
+Definition rcomp (r1 r2 : ren) : ren :=
+  fun i => r2 (r1 i).
+
+Definition rup (r : ren) : ren :=
+  rcons 0 (rcomp r rshift).
+
+(** [lift0 ofs] is a renaming which adds [ofs] to every index. *)
+Fixpoint lift0 (ofs : nat) : ren :=
+  match ofs with
+  | 0 => rid
+  | S ofs => rcomp rshift (lift0 ofs)
+  end.
+
+(** [lift base ofs] is a renaming which adds [ofs] to every index
+    greater or equal to [base]. *)
+Fixpoint lift (base ofs : nat) : ren :=
+  match base with
+  | 0 => lift0 ofs
+  | S base => rup (lift base ofs)
+  end.
+
+(** [rename r t] applies renaming [r] to term [t]. *)
+Fixpoint rename (r : ren) (t : term) : term :=
+  match t with
+  | var i => var (r i)
+  | app t1 t2 => app (rename r t1) (rename r t2)
+  | lam t => lam (rename (rup r) t)
+  | letin t u => letin (rename r t) (rename (rup r) u)
+  end.
+
+Notation "↑" := rshift.
+Notation "r1 '>>' r2" := (rcomp r1 r2) (at level 40, left associativity).
+
+(**************************************************************************)
+(** *** Names of variables. *)
+(**************************************************************************)
+
+(** A name is a unique identifier for a variable.
+    In a real implementation we would use an integer instead of a string. *)
+Definition name := string.
+
+Definition eqb_name (n n' : name) : bool :=
+  if string_dec n n' then true else false.
+
+Lemma eqb_name_spec n n' :
+  reflect (n = n') (eqb_name n n').
+Proof.
+unfold eqb_name. destruct (string_dec n n').
+- now left.
+- now right.
+Qed.
+
+Lemma eqb_name_true n : eqb_name n n = true.
+Proof. destruct (eqb_name_spec n n) ; auto. Qed.
+
+Lemma eqb_name_false n n' : n <> n' -> eqb_name n n' = false.
+Proof. intros H. destruct (eqb_name_spec n n') ; auto. now exfalso. Qed.
+
+(**************************************************************************)
+(** *** State. *)
+(**************************************************************************)
+
+Record state := mkstate {
+  d_vars : list name ; (** dest variables. *)
+  sd_ren : ren (** renaming from source to dest. *)
+}.
+
+Fixpoint lookup_var (i : nat) (x : name) (vars : list name) : nat :=
+  match vars with
+  | [] => 0 (* should not happen. *)
+  | y :: vars' =>
+    if eqb_name x y then i
+    else lookup_var (i+1) x vars'
+  end.
+
+(** Lookup the index corresponding to [x]. *)
+Definition idx_of (x : name) (s : state) : nat :=
+  lookup_var 0 x (d_vars s).
+
+Axiom fresh_name : gset name -> name.
+Axiom fresh_name_spec : forall xs, fresh_name xs ∉ xs.
+
+(**************************************************************************)
+(** *** Monadic programs. *)
+(**************************************************************************)
+
+(** Our monad [M] allows several effects:
+    - read/write access to a local context.
+    - critical failure.
+    - out of fuel, which is not considered a failure. *)
+
+Inductive result (A : Type) : Type :=
+| Success (x : A) : result A
+| Error : result A
+| OutOfFuel : result A.
+Arguments Success {A} x.
+Arguments Error {A}.
+Arguments OutOfFuel {A}.
+
+Definition M (A : Type) : Type :=
+  state -> result (state * A).
+
+Definition ret {A} (x : A) : M A :=
+  fun s => Success (s, x).
+
+Definition bind {A B} (mx : M A) (f : A -> M B) : M B :=
+  fun s =>
+    match mx s with
+    | Success (s, x) => f x s
+    | OutOfFuel => OutOfFuel
+    | Error => Error
+    end.
+
+Notation "x '>>=' f" := (bind x f) (at level 50, no associativity).
+Notation "f '=<<' x" := (bind x f) (at level 50, no associativity).
+
+(** [let*] monadic notation. *)
+Notation "'let*' x ':=' t 'in' u" := (bind t (fun x => u))
+  (at level 100, right associativity, t at next level, x pattern).
+
+Definition fmap {A B} (f : A -> B) (mx : M A) : M B :=
+  let* x := mx in
+  ret (f x).
+
+(** Signal fuel is out. *)
+Definition out_of_fuel {A} : M A := fun ctx => OutOfFuel.
+
+(** Fail. *)
+Definition error {A} : M A := fun ctx => Error.
+
+(** Read the state. *)
+Definition get : M state :=
+  fun s => Success (s, s).
+
+Definition gets {A} (f : state -> A) : M A :=
+  fun s => Success (s, f s).
+
+(** Replace the state. *)
+Definition put (s : state) : M unit :=
+  fun _ => Success (s, tt).
+
+Definition mk_var : M name :=
+  let* s := get in
+  let x := fresh_name $ list_to_set $ d_vars s in
+  let s' := mkstate (x :: d_vars s) (sd_ren s >> ↑) in
+  let* _ := put s' in
+  ret x.
+
+Definition kp_var : M name :=
+  let* s := get in
+  let x := fresh_name $ list_to_set $ d_vars s in
+  let s' := mkstate (x :: d_vars s) (rup (sd_ren s)) in
+  let* _ := put s' in
+  ret x.
+
+Definition mk_lambda (f : name -> M term) : M term :=
+  let* x := mk_var in f x.
+
+Definition kp_lambda (f : name -> M term) : M term :=
+  let* x := kp_var in f x.
+
+(**************************************************************************)
+(** *** CPS translation. *)
+(**************************************************************************)
+
+Fixpoint cps (n : nat) (t : term) (k : term) : M term :=
+  match n with 0 => out_of_fuel | S n =>
+  match t with
+  | var i => ret (app k (var i))
+  | app t1 t2 =>
+    cps n t1 =<< mk_lambda (fun x1 =>
+    (*let* r := gets sd_ren in*)
+    cps n (rename (lift0 1) t2) =<< mk_lambda (fun x2 =>
+    let* i1 := gets (idx_of x1) in
+    let* i2 := gets (idx_of x2) in
+    (*let* r := gets sd_ren in*)
+    ret (apps (var i1) [ var i2 ; rename (lift0 2) k ])))
+  | lam t' =>
+    let* body :=
+      kp_lambda (fun x =>
+      mk_lambda (fun k' =>
+      (*let* r := gets sd_ren in*)
+      let* ik' := gets (idx_of k') in
+      cps n (rename (lift0 2) t') (var ik')))
+    in
+    ret (app k body)
+  | letin t u => ret t
+    (*cps n t =<< mk_lambda (fun v =>
+    let* iv := gets (idx_of v) in
+    kk_letin (var iv) (fun x =>
+    cps n (rename (lift 1 1) u) (rename (lift0 2) k)))*)
+  end
+  end.
