theories/divergence/Coinduction_exercises.v
@@ -1,0 +1,602 @@
+From Stdlib Require Import Setoid Morphisms Lia List Nat Psatz.
+From Coinduction Require Import all.
+
+Import CoindNotations.
+Set Primitive Projections.
+Set Implicit Arguments.
+
+Module stream.
+
+(*|
+18. Streams With [coq-coinduction]: Setup
+|*)
+
+(*|
+Installation:
+- < 9.0: `opam install coq-coinduction`
+- >= 9.0: `opam install rocq-coinduction`
+-> You may have to run
+`opam repo add rocq-released https://rocq-prover.org/opam/released`
+|*)
+
+CoInductive stream := cons { hd: nat; tl: stream }.
+Declare Scope stream_scope.
+Bind Scope stream_scope with stream.
+Open Scope stream_scope.
+Infix ":::" := cons (at level 60, right associativity): stream_scope.
+
+(* We define our monotone function as before---the library provides
+   a class of complete lattices, and suitable instances for
+   (possibly dependent) relations of arbitrary arities.
+ *)
+Program Definition bisimF : mon (stream -> stream -> Prop) :=
+  {| body R s t := hd s = hd t /\ R (tl s) (tl t) |}.
+Next Obligation. firstorder. Qed.
+
+(* We use [gfp] to define the greatest fixpoint of b.
+   /!\: It has to be a notation, or we will need to unfold
+   the definition for the tactics to work.
+ *)
+Infix "~" := (gfp bisimF) (at level 70).
+Check (gfp_fp bisimF).
+Check (leq_gfp bisimF).
+
+(*|
+19. Streams: basic operations
+|*)
+
+CoFixpoint zeros: stream  := 0 ::: zeros.
+CoFixpoint zeros': stream := 0 ::: 0 ::: zeros'.
+CoFixpoint from n: stream := n ::: from (S n).
+Definition nats           := from 0.
+CoFixpoint zip s t        := hd s ::: hd t ::: zip (tl s) (tl t).
+CoFixpoint even s         := hd s ::: even (tl (tl s)).
+Definition odd s          := even (tl s).
+CoFixpoint pls s t        := hd s + hd t ::: pls (tl s) (tl t).
+Infix "+"                 := pls: stream_scope.
+
+(*|
+20. First Proofs with the [coinduction] Tactic
+|*)
+
+Goal zeros + zeros ~ zeros.
+  coinduction R CIH.
+  constructor.
+  - cbn. reflexivity.
+  - cbn. exact CIH.
+Qed.
+(*
+  coinduction R CIH.
+  constructor.
+  - reflexivity.
+  - apply CIH.
+
+  Restart.
+  now coinduction R CIH.
+Qed.*)
+
+(* Intuitively, the pairs in our coinduction candidate *)
+Infix "[~]" := (`_) (at level 70).
+(* Intuitively, the pairs that will be unlocked after a step *)
+Infix "{~}" := (bisimF `_) (at level 70).
+
+(* Go blind, restart, generalize. Draw on board the situation *)
+Lemma pls0x s: zeros + s ~ s.
+(*  coinduction R CIH.
+  split.
+  - reflexivity.
+  - cbn.
+    (* stuck *)*)
+
+  revert s. coinduction R CIH ; intros s.
+  split.
+  - reflexivity.
+  - cbn. apply CIH.
+Qed.
+
+(*|
+Exercises 1. Proofs by (vanilla) coinduction
+|*)
+
+Lemma plsC: forall x y, x + y ~ y + x.
+Proof.
+coinduction R CIH ; intros x y. split ; cbn.
+- lia.
+- apply CIH.
+Qed.
+
+Lemma plsA: forall x y z, x + (y + z) ~ (x + y) + z.
+Proof.
+coinduction R CIH ; intros x y z. split ; cbn.
+- lia.
+- apply CIH.
+Qed.
+
+Lemma even_nats: even nats ~ nats + nats.
+Proof.
+enough (forall i, even (from (2 * i)) ~ from i + from i).
+{ apply (H 0). }
+coinduction R CIH ; intros i. split ; cbn.
+- lia.
+- specialize (CIH (S i)%nat).
+  assert (2 * S i = S (S (i + (i + 0)))) as <- by lia.
+  exact CIH.
+Qed.
+
+(*|
+21. The Need for Enhanced Coinduction
+|*)
+
+Lemma bisim_refl s : s ~ s.
+Proof.
+revert s. coinduction R IH ; intros s. split.
+- reflexivity.
+- apply IH.
+Qed.
+
+Lemma unfold_stream s: s ~ hd s ::: tl s.
+Proof.
+(*  coinduction R CIH.
+  split; cbn.
+  - reflexivity.
+  - Fail apply bisim_refl. Restart.*)
+  (* Indeed, our candidate is _not_ a bisimulation. So we can strengthen it *)
+  enough (s ~ hd s ::: tl s /\ forall s, s ~ s).
+  { apply H. }
+  coinduction R CIH.
+  split.
+  - now split.
+  - split ; [reflexivity | apply CIH].
+  (* But surely, there must be a better way? *)
+Qed.
+
+(*|
+22. Enhanced Coinduction
+|*)
+
+(*|
+Coinduction principle: "any postfixpoint of [b] is below the greatest fixpoint of [b]".
+
+x <= y     y <= b y
+
+-------------------
+
+   x <= gfp b
+
+
+In the previous example, y = {s , hd s ::: tl s} was not a postfixpoint, we had to enlarge it.
+But perhaps we didn't have to?
+|*)
+
+(*|
+Let [f : X -> X] a monotone function.
+The f-enhanced coinduction principle: "any postfixpoint of [b ° f] is below the greatest fixpoint of [b]".
+
+x <= y     y <= b (f y)
+
+-------------------
+
+   x <= gfp b
+
+Of course this is completely unsound in general! Finding classes of valid [f] given a [b] has been a field of research in its own right.
+
+In the example above, we wanted to "conclude by reflexivity". That amounts to consider the up-to function [f R = R ∪ Id]. And indeed, it is sound w.r.t. bisimulation: we will prove it in a different setup a little later.
+
+|*)
+
+(*|
+Note: Beware, something can be valid of the [gfp], but not be a valid up-to.
+Famously, weak bisimilarity is transitive, but weak bisimulation up-to weak bisimilarity is not valid.
+|*)
+
+(*|
+23. Enhanced Coinduction: the Companion
+|*)
+
+(*|
+Examples:
+- Up-to reflexivity, symmetry, transitivity
+- Up-to another relation: weak bisimulation up-to strong bisimilarity, ...
+- Up-to context: for ccs, ...
+|*)
+(*|
+Historically: (prove sound and) pick the right up-to for the right proof
+|*)
+(*|
+Idea: Identify classes of sound principles that are closed under composition, etc..
+
+Definition : [f] is _(b)-compatible_ if [f ° b <= b ° f].
+Theorem    : if [f] compatible, then [f] is sound
+Theorem    : the set of b-compatible functions forms a complete lattice.
+|*)
+(*|
+The [companion] [t] of [b] is the greatest b-compatible function.
+
+We have [gfp b == t ⊥].
+We can always perform coinduction up-to [t], and access on the fly any function we prove to be below it!
+|*)
+
+(*|
+24. Enhanced Coinduction: Tower Induction
+|*)
+
+(*|
+Idea: there is a nicer, inductive, construction of the companion.
+
+We jump to [tower.v]
+|*)
+
+(*|
+25. Let's enhance!
+|*)
+
+Goal zeros + zeros ~ zeros.
+  (*coinduction R cih.
+  Undo.*)
+  apply gfp_prop.
+  intro R.
+  apply tower.
+  repeat intro; firstorder.
+(*  Restart.*)
+Abort.
+
+Instance Reflexive_t {R : Chain bisimF} : Reflexive `R.
+Proof.
+  (*revert R.
+  apply tower.
+  - cbv. firstorder.
+  - intros R HR x.
+    split.
+    + reflexivity.
+    + reflexivity.
+  (* Note: being [inf closed] does not depend on [b]! *)
+  Restart.*)
+  revert R.
+  apply Reflexive_chain. intros R HR x. now split.
+Qed.
+
+Lemma unfold_stream'' s : s ~ hd s ::: tl s.
+Proof.
+  coinduction R cih.
+  Show Proof.
+  split.
+  - reflexivity.
+  - reflexivity.
+  (* Note: we never used our coinduction hypothesis! *)
+Qed.
+
+Lemma unfold_stream''' s : s ~ hd s ::: tl s.
+Proof.
+  (* "up-to b" is always a valid principle.
+     It is captured in the tactic [step]:
+   *)
+  step.
+  split; reflexivity.
+Qed.
+
+(*|
+Exercises 2.
+|*)
+
+Goal zeros ~ zeros'.
+coinduction R CIH. split ; cbn.
+- reflexivity.
+- step. now split.
+Qed.
+
+Goal forall s, zip (even s) (odd s) ~ s.
+coinduction R CIH ; intros s. split ; cbn.
+- reflexivity.
+- step. now split.
+Qed.
+
+Lemma plusC: forall x y, x + y ~ y + x.
+Proof.
+coinduction R CIH ; intros x y. split ; cbn ; [lia|]. apply CIH.
+Qed.
+
+Lemma plus_0x x: zeros + x ~ x.
+Proof.
+revert x. coinduction R CIH ; intros x. split ; now cbn.
+Qed.
+
+Lemma plusA: forall x y z, x + (y + z) ~ (x + y) + z.
+Proof.
+coinduction R CIH ; intros x y z. split ; cbn.
+- lia.
+- apply CIH.
+Qed.
+
+(*|
+26. Let's enhance some more!
+|*)
+
+(*|
+Elements of the chain are not just reflexive, they are equivalence relations!
+|*)
+Instance Equivalence_t {R : Chain bisimF} : Equivalence `R.
+Proof.
+  constructor; revert R.
+  - apply @Reflexive_t.
+  - apply Symmetric_chain. intros R HR x y []. now split; symmetry.
+  - apply Transitive_chain. intros R HR x y z [] []. split. congruence. etransitivity; eauto.
+Qed.
+
+Lemma Equivalence_bisim : Equivalence (gfp bisimF).
+Proof. apply gfp_prop. intros R. apply Equivalence_t. Qed.
+
+(*|
+27. Shuffle Product: definition
+|*)
+
+(*|
+This is the following binary operation on streams [s,t]:
+    [(s @ t)_k = Σ_{i+j=k} (i k) s_i t_j]
+    it can be characterised by the following equations:
+    [hd (s @ t) = hd s * hd t]
+    [tl (s @ t) = tl s @ t  +  s @ tl t]
+|*)
+
+(* It's definition itself is a major challenge! *)
+Fail CoFixpoint shuf s t :=
+  (hd s * hd t) ::: (shuf (tl s) t + shuf s (tl t)).
+
+(** Here we simply assume its existence for the sake of simplicity.
+    For the curious: file [shuffle.v]
+ *)
+Parameter shuf: stream -> stream -> stream.
+Infix "@" := shuf (at level 40, left associativity).
+Axiom hd_shuf: forall s t, hd (s @ t) = (hd s * hd t)%nat.
+Axiom tl_shuf: forall s t, tl (s @ t) = tl s @ t + s @ tl t.
+Ltac cbn_shuf := repeat (rewrite ?hd_shuf, ?tl_shuf; simpl hd; simpl tl).
+
+(*|
+28. Up-to [pls] Context
+|*)
+
+Lemma shuf_0x: forall x, zeros @ x ~ zeros.
+Proof.
+  coinduction R HR. intros x. split; cbn_shuf.
+  - nia.
+  - Fail rewrite HR.
+Abort.
+
+(** addition context corresponds to a valid compatible function *)
+Instance pls_chain_proper : forall {R: Chain bisimF}, Proper (`R ==> `R ==> `R) pls.
+Proof.
+  apply (Proper_chain 2).
+  intros R HR x y [xy0 xy'] u v [uv0 uv'].
+  split; cbn.
+  - congruence.
+  - now apply HR.
+Qed.
+
+Instance pls_proper : Proper (gfp bisimF ==> gfp bisimF ==> gfp bisimF) pls.
+Proof. apply gfp_prop. intros R. apply pls_chain_proper. Qed.
+
+Lemma shuf_0x: forall x, zeros @ x ~ zeros.
+Proof.
+  coinduction R HR. intros x. split; cbn_shuf.
+  - nia.
+  - rewrite !HR. (* Uses both transitivity and up-to plus context *)
+    rewrite plus_0x.
+    reflexivity.
+Qed.
+
+(*|
+Exercises 3.
+|*)
+
+Lemma shuf_1x: forall x, zeros @ x ~ zeros.
+Admitted.
+
+Lemma shufC: forall x y, x @ y ~ y @ x.
+Proof.
+coinduction R CIH ; intros x y. split ; cbn_shuf.
+- nia.
+- rewrite (CIH (tl x) y), (CIH x (tl y)). now rewrite plsC.
+Qed.
+
+Lemma shuf_x_plus: forall x y z, x@(y + z) ~ x@y + x@z.
+Proof.
+coinduction R CIH. intros x y z. split ; cbn_shuf.
+- nia.
+- rewrite !CIH. rewrite !plsA. f_equiv. rewrite <-!plsA. f_equiv.
+  rewrite plsC. reflexivity.
+Qed.
+
+Instance shuf_proper_chain {R : Chain bisimF} : Proper (`R ==> `R ==> `R) shuf.
+Proof.
+revert R. apply (Proper_chain 2). cbn [respectful_iter].
+intros R HR x x' [Hx1 Hx2] y y' [Hy1 Hy2]. split ; cbn_shuf.
+- nia.
+- rewrite Hx2, Hy2. f_equiv.
+  + f_equiv. now step.
+  + f_equiv. now step.
+Qed.
+
+(** Not strictly needed, but might be in more complex proofs. *)
+Instance shuf_proper : Proper (gfp bisimF ==> gfp bisimF ==> gfp bisimF) shuf.
+Proof. apply gfp_prop. intros R. apply shuf_proper_chain. Qed.
+
+Lemma shuf_plus_x: forall x y z, (y + z)@x ~ y@x + z@x.
+Proof.
+intros x y z. rewrite shufC, shuf_x_plus. rewrite (shufC x y), (shufC x z).
+reflexivity.
+Qed.
+
+Lemma shufA: forall x y z, x @ (y @ z) ~ (x @ y) @ z.
+coinduction R CIH. intros x y z. split ; cbn_shuf.
+- nia.
+- rewrite shuf_plus_x, shuf_x_plus. rewrite !plsA. f_equiv ; [f_equiv|].
+  all: now rewrite CIH.
+Qed.
+
+(*|
+29. Up-to [shuffle] Context
+|*)
+
+(** shuffle product preserves the final chain *)
+(*Instance shuf_chain: forall {R: Chain bisimF}, Proper (`R ==> `R ==> `R) shuf.
+Proof.
+  apply (Proper_chain 2).
+  intros R HR x y [xy xy'] u v [uv uv'].
+  split; cbn_shuf.
+  - congruence.
+  - now rewrite xy', uv', xy, uv.
+Qed.*)
+
+(*|
+30. Accumulate
+|*)
+
+(*|
+One can build the coinduction candidate on the fly.
+
+Initially introduced in paco:
+G b x := gfp (λy . b (x ∪ y))
+
+accumulate: y <= G b x <-> y <= G b (x ∪ y)
+
+Intuition: it is sound to record pairs we have encountered as valid stopping point, if we keep going first.
+
+|*)
+
+Goal zeros ~ zeros'.
+Proof.
+  coinduction R cih.
+  split; [reflexivity |].
+  accumulate cih'.
+  split; [reflexivity |].
+  exact cih.
+Qed.
+
+(*|
+Note: Once you move to a principle rich enough to support clean
+up-to [b], use cases become more rare.
+|*)
+
+(*|
+|*)
+
+(** * convolution product *)
+
+CoFixpoint c n := n ::: c n.
+
+(** this is the following binary operation on streams [s,t]:
+    [(s*t)_k = Σ_{i+j=k} s_i t_j]
+    (note that the binomial coefficient has disappeared)
+
+    it can be characterised by the following equations:
+    [hd (s*t) = hd s * hd t]
+    [tl (s*t) = tl s * t + hd s ** tl t]
+    There [**] is pointwise multiplication by a scalar, which is a special case of convolution product:
+    [x ** s = c x * s]
+    (Remember that [c x] is the stream [x,0,0,...] )
+ *)
+
+(** Like before, we cannot define it as one could expect in Coq,
+    because of the guard condition: *)
+Fail CoFixpoint mult s t :=
+  cons (hd s * hd t)%nat (mult (tl s) t + mult (c (hd s)) (tl t)).
+
+(** Here we simply assume its existence for the sake of simplicity. *)
+Parameter mult: stream -> stream -> stream.
+Infix "*" := mult.
+Axiom hd_mult: forall s t, hd (s * t) = (hd s * hd t)%nat.
+Axiom tl_mult: forall s t, tl (s * t) = tl s * t + c (hd s) * tl t.
+Ltac cbn_mult := repeat (rewrite ?hd_mult, ?tl_mult; simpl hd; simpl tl).
+
+Lemma mult_0x: forall x, c 0 * x ~ c 0.
+Proof.
+Admitted.
+
+Lemma mult_x0: forall x, x  * c 0 ~ c 0.
+Proof.
+Admitted.
+
+Lemma mult_1x: forall x, c 1 * x ~ x.
+Proof.
+Admitted.
+
+Lemma mult_x1: forall x, x * c 1 ~ x.
+Proof.
+Admitted.
+
+Lemma mult_x_plus: forall x y z, x * (y + z) ~ x*y + x*z.
+Proof.
+Admitted.
+
+Lemma c_plus n m: c (n+m) ~ c n + c m.
+Proof.
+Admitted.
+
+Lemma c_mult n m: c (n*m) ~ c n * c m.
+Proof.
+Admitted.
+
+(** convolution product preserves the final chain  *)
+Instance mult_chain: forall {R: Chain bisimF}, Proper (`R ==> `R ==> `R) mult.
+Proof.
+Admitted.
+
+Lemma mult_plus_x: forall x y z, (y + z) * x ~ y*x + z*x.
+Proof.
+Admitted.
+
+Lemma multA: forall x y z, x * (y * z) ~ (x * y) * z.
+Proof.
+Admitted.
+
+(** below: commutativity of convolution product, following Rutten's
+    proof *)
+
+Lemma multC_n n: forall x, c n * x ~ x * c n.
+Proof.
+Admitted.
+
+Definition X := cons 0 (c 1).
+
+Theorem expand x: x ~ c (hd x) + X * tl x.
+Proof.
+Admitted.
+
+Lemma multC_11 x: tl (X * x) ~ x.
+Proof.
+Admitted.
+
+Lemma multC_X: forall x, X * x ~ x * X.
+Proof.
+Admitted.
+
+Lemma multC: forall x y, x * y ~ y * x.
+Proof.
+Admitted.
+
+End stream.
+
+(*|
+31. Going Further
+|*)
+
+(*|
+Library support for coinductive relations and proofs by coinduction!
+
+But what about coinductive types and corecursive programming?
+Some help to define the shuffle product?
+
+You can do it smoothly in Isabelle/HOL!
+
+~> A library of final coalgebras and up-to corecursion?
+For the curious reader, some introductory elements in this direction can be found here: https://github.com/damien-pous/epit25/
+|*)
+
+(*|
+More examples?
+
+- Tutorial examples: https://github.com/damien-pous/coinduction-examples
+
+- Real world example with [paco] : https://github.com/DeepSpec/InteractionTrees
+
+- Real world example with [coinduction] : https://github.com/vellvm/ctrees
+|*)
