theories/divergence/FuelFreeMonad.v
@@ -1,0 +1,349 @@
+From Stdlib Require Import Bool Nat Lia Classes.Morphisms.
+
+(**************************************************************************)
+(** *** Monadic programs. *)
+(**************************************************************************)
+
+Axiom context : Type.
+
+Inductive M_ : Type -> Type :=
+| Ret {A} : A -> M_ A
+| Bind {A B} : M_ A -> (A -> M_ B) -> M_ B
+| GetCtx : M_ context
+| PutCtx : context -> M_ unit
+| Fail {A} : M_ A
+| OutOfFuel {A} : M_ A.
+
+Definition M A :=
+  nat -> M_ A.
+
+Definition ret {A} (x : A) : M A :=
+  fun _ => Ret x.
+
+Definition bind {A B} (m : M A) (f : A -> M B) : M B :=
+  fun n => Bind (m n) (fun x => f x n).
+
+(** [let*] monadic notation. *)
+Notation "'let*' x ':=' t 'in' u" := (bind t (fun x => u))
+  (at level 100, right associativity, t at next level, x pattern).
+
+Definition fmap {A B} (f : A -> B) (m : M A) : M B :=
+  let* x := m in
+  ret (f x).
+
+Notation "f <$> x" := (fmap f x) (at level 30, right associativity).
+
+Definition get_ctx : M context :=
+  fun _ => GetCtx.
+
+Definition put_ctx c : M unit :=
+  fun _ => PutCtx c.
+
+Definition fail {A} : M A :=
+  fun _ => Fail.
+
+Definition out_of_fuel {A} : M A :=
+  fun _ => OutOfFuel.
+
+(** Fixpoint combinator. *)
+Fixpoint fix1 {A B} (F : (A -> M B) -> (A -> M B)) (x : A) (n : nat) : M_ B :=
+  match n with
+  | 0 => OutOfFuel
+  | S n => F (fun x' _ => fix1 F x' n) x n
+  end.
+
+(** Example: factorial function. *)
+Definition fact : nat -> M nat :=
+  fix1 (fun fact k =>
+    match k with
+    | 0 => ret 1
+    | S k => mult (S k) <$> fact k
+    end).
+
+(**************************************************************************)
+(** *** Program semantics (as a monadic interpreter). *)
+(**************************************************************************)
+
+Inductive result A :=
+| RSuccess (x : A)
+| RFail
+| ROutOfFuel.
+
+Arguments RSuccess {A}.
+Arguments RFail {A}.
+Arguments ROutOfFuel {A}.
+
+Fixpoint run_ {A} (m : M_ A) (c : context) : result (context * A) :=
+  match m with
+  | Ret x => RSuccess (c, x)
+  | Bind m f =>
+    match run_ m c with
+    | RSuccess (c', x) => run_ (f x) c'
+    | RFail => RFail
+    | ROutOfFuel => ROutOfFuel
+    end
+  | GetCtx => RSuccess (c, c)
+  | PutCtx c' => RSuccess (c', tt)
+  | Fail => RFail
+  | OutOfFuel => ROutOfFuel
+  end.
+
+(**************************************************************************)
+(** *** (Partial) program logic. *)
+(**************************************************************************)
+
+Definition wp_result {A} (r : result (context * A)) (Φ : A -> context -> Prop) : Prop :=
+  match r with
+  | RSuccess (c, x) => Φ x c
+  | RFail => False
+  | ROutOfFuel => True
+  end.
+
+(** A weakest precondition which does not require termination. *)
+Definition wp {A} (m : M A) (c : context) (Φ : A -> context -> Prop) : Prop :=
+  forall n, wp_result (run_ (m n) c) Φ.
+
+(** Hoare triples. *)
+Definition hoare {A} (P : context -> Prop) (m : M A) (Q : A -> context -> Prop) :=
+  forall c, P c -> wp m c Q.
+
+Lemma wp_result_consequence {A} Φ Φ' (r : result (context * A)) :
+  wp_result r Φ ->
+  (forall x c, Φ x c -> Φ' x c) ->
+  wp_result r Φ'.
+Proof. intros H HΦ. destruct r as [[] | |] ; cbn in * ; auto. Qed.
+
+Lemma wp_consequence {A} Φ Φ' (m : M A) c :
+  wp m c Φ ->
+  (forall x c, Φ x c -> Φ' x c) ->
+  wp m c Φ'.
+Proof.
+intros H HΦ n. eapply wp_result_consequence.
+- apply H.
+- apply HΦ.
+Qed.
+
+Lemma wp_ret {A} (a : A) c Φ :
+  Φ a c -> wp (ret a) c Φ.
+Proof. intros H n. cbn. assumption. Qed.
+
+(** The converse implication might not be true? *)
+Lemma wp_bind {A B} (m : M A) (f : A -> M B) c Φ :
+  wp m c (fun x c' => wp (f x) c' Φ) -> wp (bind m f) c Φ.
+Proof.
+intros H n. cbn. specialize (H n). unfold wp_result in *.
+destruct (run_ (m n) c) as [[] | |] ; auto. apply H.
+Qed.
+
+Lemma wp_get_ctx c Φ :
+  Φ c c -> wp get_ctx c Φ.
+Proof. intros H n. cbn. assumption. Qed.
+
+Lemma wp_put_ctx c c' Φ :
+  Φ tt c' -> wp (put_ctx c') c Φ.
+Proof. intros H n. cbn. assumption. Qed.
+
+Lemma wp_out_of_fuel {A} c Φ :
+  wp (@out_of_fuel A) c Φ.
+Proof. intros n. cbn. constructor. Qed.
+
+Lemma hoare_fix1 {A B} (F : (A -> M B) -> (A -> M B))
+  (P : A -> context -> Prop) (Q : A -> B -> context -> Prop) :
+  (forall f,
+    (forall x, hoare (P x) (f x) (Q x)) ->
+    (forall x, hoare (P x) (F f x) (Q x))) ->
+  forall x, hoare (P x) (fix1 F x) (Q x).
+Proof.
+cbn. intros HF x c Hx n. induction n in c, x, Hx, HF, c, P, Q |- * ; cbn.
+- constructor.
+- apply HF ; [|exact Hx]. intros c' x' Hx' _. eapply IHn ; eassumption.
+Qed.
+
+(** Example: proving a simple property of factorial. *)
+Lemma fact_pos :
+  forall k, hoare (fun _ => True) (fact k) (fun res _ => max 1 k <= res).
+Proof.
+apply hoare_fix1 with (P := fun _ _ => True) (Q := fun k res _ => max 1 k <= res).
+intros f Hf k c _. destruct k.
+- apply wp_ret. lia.
+- apply wp_bind. eapply wp_consequence ; [now apply Hf|].
+  intros k' c'' Hk'. cbn beta in Hk'. apply wp_ret.
+  assert (1 <= k') by lia. lia.
+Qed.
+
+(**************************************************************************)
+(** *** Monotonicity. *)
+(**************************************************************************)
+
+(** Partial order relation on [result A]. *)
+Inductive lessdefR {A} : result A -> result A -> Prop :=
+| lessdefR_oof x : lessdefR ROutOfFuel x
+| lessdefR_fail : lessdefR RFail RFail
+| lessdefR_suc a : lessdefR (RSuccess a) (RSuccess a).
+
+#[export] Instance lessdefR_preorder A : PreOrder (@lessdefR A).
+Proof.
+constructor.
+- intros [] ; constructor.
+- intros r1 r2 r3 H1 H2. destruct r1.
+  + destruct r2 ; inversion H1 ; subst. assumption.
+  + destruct r2 ; inversion H1 ; subst. assumption.
+  + constructor.
+Qed.
+
+(** Partial order relation on [M_ A]. *)
+Definition lessdef_ {A} (m m' : M_ A) :=
+  forall c, lessdefR (run_ m c) (run_ m' c).
+
+#[export] Instance lessdef__preorder A : PreOrder (@lessdef_ A).
+Proof.
+constructor.
+- intros m c. reflexivity.
+- intros m1 m2 m3 H1 H2 c. etransitivity ; eauto.
+Qed.
+
+(** Partial order relation on [M A]. *)
+Definition lessdef {A} (m m' : M A) := forall n, lessdef_ (m n) (m' n).
+Notation "m ⊑ m'" := (lessdef m m') (at level 50, no associativity).
+
+Definition lessdef1 {A B} (f f' : A -> M B) := forall x, lessdef (f x) (f' x).
+Notation "f ⊑₁ g" := (lessdef1 f g) (at level 50, no associativity).
+
+#[export] Instance lessdef_preorder A : PreOrder (@lessdef A).
+Proof.
+constructor.
+- intros m n. reflexivity.
+- intros m1 m2 m3 H1 H2 n. etransitivity ; eauto.
+Qed.
+
+(** Monotonicity. *)
+Definition mono {A} (m : M A) :=
+  forall n n', n <= n' -> lessdef_ (m n) (m n').
+
+Definition mono1 {A B} (f : A -> M B) :=
+  forall x, mono (f x).
+
+(** Proving monotonicity. *)
+
+Lemma ret_mono {A} (a : A) :
+  mono (ret a).
+Proof. intros n n' Hn c. cbn. constructor. Qed.
+
+Lemma bind_mono {A B} (m : M A) (f : A -> M B) :
+  mono m -> mono1 f -> mono (bind m f).
+Proof.
+intros Hm Hf n n' Hn c. cbn. specialize (Hm n n' Hn c).
+destruct (run_ (m n) c) as [[] | |] ; destruct (run_ (m n') c) as [[] | |].
+all: try solve [ constructor | now inversion Hm ].
+inversion Hm ; subst. now apply Hf.
+Qed.
+
+Lemma fmap_mono {A B} (f : A -> B) (m : M A) :
+  mono m -> mono (f <$> m).
+Proof.
+intros H. unfold fmap. apply bind_mono.
+- assumption.
+- intros x. apply ret_mono.
+Qed.
+
+Lemma get_ctx_mono : mono get_ctx.
+Proof. intros n n' Hn c. cbn. constructor. Qed.
+
+Lemma put_ctx_mono c : mono (put_ctx c).
+Proof. intros n n' Hn c'. cbn. constructor. Qed.
+
+Lemma fail_mono A : mono (@fail A).
+Proof. intros n n' Hn c. cbn. constructor. Qed.
+
+Lemma out_of_fuel_mono A : mono (@out_of_fuel A).
+Proof. intros n n' Hn c. cbn. constructor. Qed.
+
+Lemma fix1_mono {A B} (F : (A -> M B) -> (A -> M B)) :
+  (forall f, mono1 f -> mono1 (F f)) ->
+  (forall f g : A -> M B, f ⊑₁ g -> F f ⊑₁ F g) ->
+  mono1 (fix1 F).
+Proof.
+intros H1 H2 x n n' Hn. induction n in x, n', Hn |- * ; cbn.
+- constructor.
+- destruct n' ; cbn ; [lia|]. transitivity (F (fun x' _ => fix1 F x' n') x n).
+  + apply H2. intros y _. apply IHn. lia.
+  + apply H1.
+    * intros y _ _ _. reflexivity.
+    * lia.
+Qed.
+
+Lemma bind_lessdef {A B} :
+  Proper (lessdef ==> lessdef1 ==> lessdef) (@bind A B).
+Proof.
+intros m m' Hm f f' Hf n c. cbn. specialize (Hm n c).
+destruct (run_ (m n) c) as [[] | |] ; destruct (run_ (m' n) c) as [[] | |].
+all: try solve [ constructor | now inversion Hm ].
+inversion Hm ; subst. apply Hf.
+Qed.
+
+Lemma fmap_lessdef {A B} (f : A -> B) :
+  Proper (lessdef ==> lessdef) (fmap f).
+Proof.
+intros m m' Hm. unfold fmap. apply bind_lessdef.
+- assumption.
+- intros x. reflexivity.
+Qed.
+
+(** Prove goals of the form [mono _] or [_ ⊑ _]. *)
+Ltac prove_mono :=
+  match goal with
+  (* Introduce variables. *)
+  | [ |- mono1 _ ] => intro ; prove_mono
+  | [ |- _ ⊑₁ _ ] => intro ; prove_mono
+  (* [lessdef] rules. *)
+  | [ |- ?x ⊑ ?x] => reflexivity
+  | [ |- bind _ _ ⊑ bind _ _ ] => apply bind_lessdef ; [prove_mono | prove_mono]
+  | [ |- fmap _ _ ⊑ fmap _ _ ] => apply fmap_lessdef ; [prove_mono]
+  (* Monotonicity rules. *)
+  | [ |- mono (ret _) ] => apply ret_mono
+  | [ |- mono (bind _ _) ] => apply bind_mono ; [prove_mono | prove_mono]
+  | [ |- mono (fmap _ _) ] => apply fmap_mono ; [prove_mono]
+  | [ |- mono (fix1 _ _) ] =>
+      apply fix1_mono ; [intro ; intro ; prove_mono | intro ; intro ; intro ; prove_mono]
+  (* Try to use assumptions. *)
+  | [ H : mono _ |- mono _ ] => exact H
+  | [ H : mono1 _ |- mono _ ] => apply H
+  | [ H : _ ⊑ _ |- _ ⊑ _ ] => exact H
+  | [ H : _ ⊑₁ _ |- _ ⊑ _ ] => apply H
+  (* Break up case expressions. *)
+  | [ |- mono (match ?x with _ => _ end) ] => destruct x ; prove_mono
+  | [ |- (match ?x with _ => _ end) ⊑ (match ?x with _ => _ end) ] =>
+      destruct x ; prove_mono
+  (* Otherwise give up. *)
+  | _ => idtac
+  end.
+
+(** Example: fact is monotone. *)
+Lemma fact_mono :
+  mono1 fact.
+Proof. unfold fact. prove_mono. Qed.
+
+(**************************************************************************)
+(** *** Termination. *)
+(**************************************************************************)
+
+Definition is_out_of_fuel {A} (m : M_ A) : Prop :=
+  match m with
+  | OutOfFuel => True
+  | _ => False
+  end.
+
+Definition terminates {A} (m : M A) :=
+  exists n, ~is_out_of_fuel (m n).
+
+Definition diverges {A} (m : M A) :=
+  forall n, is_out_of_fuel (m n).
+
+Lemma ret_terminates {A} (a : A) :
+  terminates (ret a).
+Proof. exists 0. cbn. auto. Qed.
+
+Lemma bind_terminates {A B} (m : M A) (f : A -> M B) :
+  terminates (bind m f).
+Proof.
+intros [n Hm] Hf. eexists. cbn.
